***NO_CI** patch proposition for jake

examples/data_structures/graph/Graph.Search.fst
@@ -14,7 +14,7 @@ module MC = Map.Complements
 let lemma_reachable_trans (#n:nat) (g:graph0 n) (n1 n2 n3:fin n)
  : Lemma (requires (reachable g n1 n2) /\ (reachable g n2 n3))
  (ensures (reachable g n1 n3))
- = 
+ =
    let aux (p1 p2 : path g) : Lemma (requires (from p1 == n1 /\ to p1 == n2) /\ (from p2 == n2 /\ to p2 == n3) ) (ensures (reachable g n1 n3)) =
      let _ = append g p1 p2 in ()
    in
@@ -24,7 +24,7 @@ let lemma_reachable_trans (#n:nat) (g:graph0 n) (n1 n2 n3:fin n)
 
 let rec bfs_aux (#n:nat) (g:graph0 n{no_parallel_edge g}) (s:nodeset n) (f:nodeset n)
  : Pure (nodeset n)
- (requires (True) 
+ (requires (True)
   /\ N.disjoint s f)
  (ensures (fun p' -> True ))
  (decreases %[n - L.length  s])
@@ -51,63 +51,71 @@ let bfs (#n:nat) (g:graph0 n{no_parallel_edge g}) (node : fin n) =
 
 let decrease_clause (n:nat) (s:nodeset n) : nat = LC.noRepeats_length_lemma s ; n - L.length s
 
+let neither_in (#n0:nat) (l1 l2: nodeset n0) n = not (L.mem n l1) && not (L.mem n l2)
+
+let fill_map #a #b (m:M.t a b) (l:list a) (v:b) =
+  L.fold_left (fun acc i -> M.upd acc i v) m l
+
 let rec bfs_map_aux (#n:nat) (g:graph0 n{no_parallel_edge g}) (seen:nodeset n) (frntr:nodeset n) (parents:M.t (fin n) (fin n))
  : Pure (nodeset n * M.t (fin n) (fin n))
  (requires  N.disjoint seen frntr)
  (ensures (fun p' -> True ))
  (decreases (decrease_clause n seen))
- = match frntr with
- | [] -> seen, parents
- | hd :: tl ->
-  let adj = g @^ hd in
-  let neither_in_s_nor_f n = not (L.mem n seen) && not (L.mem n frntr) in
-  let adj_unscene = L.filter neither_in_s_nor_f adj in
-  LC.noRepeats_filter neither_in_s_nor_f adj;
-  
-  let s' = hd :: seen in
-  let f' = N.append tl adj_unscene in
-  let p' = L.fold_left (fun acc i -> M.upd acc i hd) parents adj_unscene in
+= match frntr with
+  | [] -> seen, parents
+  | hd :: tl ->
+    let adj = g @^ hd in
+    let neither_in_s_nor_f = neither_in seen frntr in
+    let adj_unscene = L.filter neither_in_s_nor_f adj in
+    LC.noRepeats_filter neither_in_s_nor_f adj;
 
-  N.lemma_disjoint_append tl adj_unscene s';
-(*  noRepeats_length_lemma (s');  *)
-  bfs_map_aux g s' f' p'
+    let s' = hd :: seen in
+    let f' = N.append tl adj_unscene in
+    let p' = fill_map parents adj_unscene hd in
 
+    N.lemma_disjoint_append tl adj_unscene s';
+    bfs_map_aux g s' f' p'
 
+let parent_map_valid (#n:nat) (g:graph0 n) (parents:M.t (fin n) (fin n)) =
+  forall (x : fin n) . M.contains parents x ==>  is_in_graph (M.sel parents x) x g
+
+#set-options "--detail_errors"
 
 let rec lemma_bfs_map_pairing_aux (#n:nat) (g:graph0 n{no_parallel_edge g}) (seen:nodeset n) (frntr:nodeset n) (parents:M.t (fin n) (fin n))
- : Lemma 
-   (requires N.disjoint seen frntr /\
-     (forall (x : fin n) . M.contains parents x ==>  is_in_graph (M.sel parents x) x g) /\
-   (forall (x: fin n) . L.mem x seen || L.mem x frntr <==> M.contains parents x))
- 
-   (ensures N.disjoint seen frntr /\
-   (let s', p' = bfs_map_aux g seen frntr parents in (forall (x : fin n) . M.contains p' x ==>  is_in_graph (M.sel p' x) x g)))
-   (decreases (decrease_clause n seen))
- = match frntr with
- | [] -> admit()
- | hd :: tl ->
+ : Lemma
+   (requires
+     N.disjoint seen frntr /\
+     parent_map_valid g parents /\
+     (forall (x: fin n) . L.mem x seen || L.mem x frntr <==> M.contains parents x))
 
-  let adj = g @^ hd in
-  let neither_in_s_nor_f n = not (L.mem n seen) && not (L.mem n frntr) in
-  let adj_unscene = L.filter neither_in_s_nor_f adj in
-  LC.noRepeats_filter neither_in_s_nor_f adj;
-  
-  let s' = hd :: seen in
-  let f' = N.append tl adj_unscene in
-  let p' = L.fold_left (fun acc i -> M.upd acc i hd) parents adj_unscene in
-  assume((forall (x: fin n) . L.mem x s' || L.mem x f'  <==> M.contains p' x));
-  assume(N.disjoint s' f');
-  assume((forall (x : fin n) . M.contains p' x ==>  is_in_graph (M.sel p' x) x g));
-  
-  lemma_bfs_map_pairing_aux g s' f' p'
+   (ensures N.disjoint seen frntr /\
+     (let s', p' = bfs_map_aux g seen frntr parents in parent_map_valid g p'))
+   (decreases (decrease_clause n seen))
+= match frntr with
+  | [] -> admit()
+  | hd :: tl ->
+    let adj = g @^ hd in
+    let neither_in_s_nor_f = neither_in seen frntr in
+    let adj_unscene = L.filter neither_in_s_nor_f adj in
+    LC.noRepeats_filter neither_in_s_nor_f adj;
+
+    let s' = hd :: seen in
+    let f' = N.append tl adj_unscene in
+    let p' = fill_map parents adj_unscene hd in
+    assume((forall (x: fin n) . L.mem x s' || L.mem x f'  <==> M.contains p' x));
+    assume(N.disjoint s' f');
+    assume((forall (x : fin n) . M.contains p' x ==>  is_in_graph (M.sel p' x) x g));
+    assert (bfs_map_aux g seen frntr parents == bfs_map_aux g s' f' p') ;
+
+    lemma_bfs_map_pairing_aux g s' f' p'
 
 
 let rec lemma_bfs_map_pairing_aux2 (#n:nat) (g:graph0 n{no_parallel_edge g}) (seen:nodeset n) (frntr:nodeset n) (parents:M.t (fin n) (fin n)) (si : nodeset n) (fi : nodeset n) (pi:M.t (fin n) (fin n))
- : Lemma 
-   (requires N.disjoint seen frntr /\ N.disjoint si fi /\ 
+ : Lemma
+   (requires N.disjoint seen frntr /\ N.disjoint si fi /\
    (forall (x : fin n) . M.contains parents x ==>  is_in_graph (M.sel parents x) x g) /\
    (forall (x: fin n) . L.mem x seen || L.mem x frntr <==> M.contains parents x))
-   (ensures N.disjoint si fi /\ 
+   (ensures N.disjoint si fi /\
    (let s', p' = bfs_map_aux g si fi pi in s' == seen /\ p' == parents /\(forall (x : fin n) . M.contains p' x ==>  is_in_graph (M.sel p' x) x g)))
    (decreases (decrease_clause n seen))
  = match frntr with
@@ -118,7 +126,7 @@ let rec lemma_bfs_map_pairing_aux2 (#n:nat) (g:graph0 n{no_parallel_edge g}) (se
   let neither_in_s_nor_f n = not (L.mem n seen) && not (L.mem n frntr) in
   let adj_unscene = L.filter neither_in_s_nor_f adj in
   LC.noRepeats_filter neither_in_s_nor_f adj;
-  
+
   let s' = hd :: seen in
   let f' = N.append tl adj_unscene in
   let p' = L.fold_left (fun acc i -> M.upd acc i hd) parents adj_unscene in
@@ -139,11 +147,11 @@ let rec lemma_bfs_map_pairing_aux2 (#n:nat) (g:graph0 n{no_parallel_edge g}) (se
 
   MC.domain_lemma2 parents adj_unscene (fun _ -> hd);
   assert(forall (x : fin n) . L.mem x seen || L.mem x adj_unscene ==> M.contains p' x);
-  
+
   assert(forall (x : fin n) . M.contains p' x ==>  is_in_graph (M.sel p' x) x g);
 *)
   assume((forall (x: fin n) . L.mem x s' || L.mem x f'  <==> M.contains p' x));
   assume(N.disjoint s' f');
   assume((forall (x : fin n) . M.contains p' x ==>  is_in_graph (M.sel p' x) x g));
-  
+
   lemma_bfs_map_pairing_aux2 g s' f' p' si fi pi
